SimAsm/SimAsm_Rules.thy
@@ -2,57 +2,104 @@ theory SimAsm_Rules
   imports SimAsm_StateStack SimAsm_Reasoning 
   begin
 
-lift_definition tstack_flat :: "('r,'v,'a) tstack \<Rightarrow> ('r,'v,'a) varmap'" 
-  is "\<lambda>s. \<lparr> varmap_st = tlookup s, \<dots> = frame.more (hd (Rep_tstack s))\<rparr>".
+lift_definition vm_of_ts :: "('r,'v,'a) tstack \<Rightarrow> ('r,'v,'a) varmap'" 
+  is "\<lambda>s. \<lparr> varmap_st = tlookup s, \<dots> = frame.more (last (Rep_tstack s))\<rparr>".
 
-lift_definition tstack_pred :: "('r,'v,'a) varmap' pred \<Rightarrow> ('r,'v,'a) tstack pred" is
-  "\<lambda>v. tstack_flat -` v".
+lift_definition ts_of_vm :: "('r,'v,'a) varmap' \<Rightarrow> ('r,'v,'a) tstack" 
+  is "inv vm_of_ts".
+
+lemma ts_of_vm_exists: "\<exists>ts. vm_of_ts ts = vm"
+proof
+  let ?s = "[\<lparr> frame_st = Some \<circ> varmap_st vm, frame_cap = UNIV, \<dots> = more vm \<rparr>]"
+  let ?ts = "Abs_tstack ?s"
+  have "Is_tstack ?s" by (simp add: Is_tstack_def)
+  hence 1: "RepAbs_tstack ?s = ?s" by simp
+  show "vm_of_ts ?ts = vm" 
+    unfolding vm_of_ts_def tlookup_def 
+    apply (simp add: 1) 
+    unfolding lookup.simps by simp
+    qed
   
-lift_definition tstack_rel :: "('r,'v,'a) varmap' rel \<Rightarrow> ('r,'v,'a) tstack rel" is 
-  "\<lambda>x. {(s,s') | s s'. (tstack_flat s, tstack_flat s') \<in> x}".
-  
-fun tstack_com :: "('r,'v,('r,'v,'a)varmap','a) lang \<Rightarrow> ('r, 'v, ('r, 'v, 'a) tstack, 'a) lang" where
-  "tstack_com (Skip) = Skip " |
-  "tstack_com (Op pred op auxfn) = Op (tstack_pred pred) op (auxfn \<circ> tstack_flat)" |
-  "tstack_com (Seq a b) = Seq (tstack_com a) (tstack_com b) " |
-  "tstack_com (If c t f) = If c (tstack_com t) (tstack_com f)" |
-  "tstack_com (While b Imix Ispec c) = While b (tstack_pred Imix) (tstack_pred Ispec) (tstack_com c) " |
-  "tstack_com (DoWhile Imix Ispec c b) = DoWhile (tstack_pred Imix) (tstack_pred Ispec) (tstack_com c) b "
- 
-
-context reasoning_spec
-begin
-print_locale reasoning_spec
-print_locale wp_spec
-
-
-interpretation srules: rules undefined tstack_push
-proof (unfold_locales, standard)
-  fix m s m' s'
-  assume "tstack_push m s = tstack_push m' s'" 
-  hence 1: 
-    "Abs_tstack (\<lparr>frame_st = frame_st s, frame_cap = frame_cap s, \<dots> = undefined\<rparr> # Rep_tstack m) 
-    = Abs_tstack (\<lparr>frame_st = frame_st s', frame_cap = frame_cap s', \<dots> = undefined\<rparr> # Rep_tstack m')"
-    (is "Abs_tstack ?L = Abs_tstack ?R")
-    unfolding tstack_push_def by simp
-  let "?s # Rep_tstack m" = ?L
-  let "?s' # Rep_tstack m'" = ?R
-  from 1 have Is_tstack: "Is_tstack ?L" "Is_tstack ?R" "Is_tstack (Rep_tstack m)" "Is_tstack (Rep_tstack m')" 
-    by auto
-  hence "?s = ?s'" "Rep_tstack m = Rep_tstack m'" using 1 RepAbs_id list.inject by metis+
-  show "s = s'" using \<open>?s = ?s'\<close> using frame.equality frame.ext_inject by (metis (full_types) unit.exhaust)
-  show "m = m'" using \<open>Rep_tstack m = Rep_tstack m'\<close> Rep_tstack_inject by auto
+lemma ts_of_vm_inverse: "vm_of_ts (ts_of_vm vm) = vm"
+proof -
+  have a: "ts_of_vm vm = (SOME ts. vm_of_ts ts = vm)" 
+    by (simp add: inv_def ts_of_vm.abs_eq)
+  have "varmap_st vm = tlookup (ts_of_vm vm)" 
+    using a ts_of_vm_exists
+    by (metis (mono_tags, lifting) varmap_rec.select_convs(1) verit_sko_ex' vm_of_ts.transfer)  
+  moreover have "more vm = frame.more (last (Rep_tstack (ts_of_vm vm)))"
+    using a ts_of_vm_exists
+    by (metis (mono_tags, lifting) varmap_rec.select_convs(2) verit_sko_ex' vm_of_ts.transfer)    
+  ultimately show ?thesis unfolding vm_of_ts_def by simp
 qed
+  
+lift_definition ts_pred_of_vm_pred :: "('r,'v,'a) varmap' pred \<Rightarrow> ('r,'v,'a) tstack pred" is
+  "\<lambda>v. vm_of_ts -` v".
+  
+lift_definition ts_rel_of_vm_rel :: "('r,'v,'a) varmap' rel \<Rightarrow> ('r,'v,'a) tstack rel" is 
+  "\<lambda>x. {(s,s') | s s'. (vm_of_ts s, vm_of_ts s') \<in> x}".
+  
+fun ts_lang_of_vm_lang :: "('r,'v,('r,'v,'a)varmap','a) lang \<Rightarrow> ('r, 'v, ('r, 'v, 'a) tstack, 'a) lang" where
+  "ts_lang_of_vm_lang (Skip) = Skip " |
+  "ts_lang_of_vm_lang (Op pred op auxfn) = Op (ts_pred_of_vm_pred pred) op (auxfn \<circ> vm_of_ts)" |
+  "ts_lang_of_vm_lang (Seq a b) = Seq (ts_lang_of_vm_lang a) (ts_lang_of_vm_lang b) " |
+  "ts_lang_of_vm_lang (If c t f) = If c (ts_lang_of_vm_lang t) (ts_lang_of_vm_lang f)" |
+  "ts_lang_of_vm_lang (While b Imix Ispec c) = While b (ts_pred_of_vm_pred Imix) (ts_pred_of_vm_pred Ispec) (ts_lang_of_vm_lang c) " |
+  "ts_lang_of_vm_lang (DoWhile Imix Ispec c b) = DoWhile (ts_pred_of_vm_pred Imix) (ts_pred_of_vm_pred Ispec) (ts_lang_of_vm_lang c) b "
 
-term rules.rules
+fun vm_lang_of_ts_lang :: "('r,'v,('r,'v,'a)tstack,'a) lang \<Rightarrow> ('r, 'v, ('r, 'v, 'a) varmap', 'a) lang" where
+  "vm_lang_of_ts_lang (Skip) = Skip " |
+  "vm_lang_of_ts_lang (Op pred op auxfn) = Op (vm_of_ts ` pred) op (auxfn \<circ> ts_of_vm)" |
+  "vm_lang_of_ts_lang (Seq a b) = Seq (vm_lang_of_ts_lang a) (vm_lang_of_ts_lang b) " |
+  "vm_lang_of_ts_lang (If c t f) = If c (vm_lang_of_ts_lang t) (vm_lang_of_ts_lang f)" |
+  "vm_lang_of_ts_lang (While b Imix Ispec c) = While b (vm_of_ts ` Imix) (vm_of_ts ` Ispec) (vm_lang_of_ts_lang c) " |
+  "vm_lang_of_ts_lang (DoWhile Imix Ispec c b) = DoWhile (vm_of_ts ` Imix) (vm_of_ts ` Ispec) (vm_lang_of_ts_lang c) b "
 
+  
+locale simasm_rules = 
+  reasoning_spec 
+    where st = tlookup
+    and st_upd = tupdate
+    and aux = taux
+    and aux_upd = tauxupd
+    and rg = rg 
+    and glb = glb
+  + rules 
+    where exists_act = "undefined :: ('r,'v,'a) auxopSt"
+    and push = "tstack_push :: ('r,'v,'a) tstack \<Rightarrow> ('r,'v) frame \<Rightarrow> ('r,'v,'a) tstack"
+  for st :: "('r,'v,'a) tstack \<Rightarrow> 'r \<Rightarrow> 'v"
+  and rg :: "('r,'v,'a) varmap' \<Rightarrow> ('r,'v,'a) varmap'"
+  and glb :: "('r,'v,'a) varmap' \<Rightarrow> ('r,'v,'a) varmap'"
+  
+context simasm_rules
+begin
+
+(* interpretation srules: rules undefined tstack_push *)
+(* proof (unfold_locales, standard) *)
+  (* fix m s m' s' *)
+  (* assume "tstack_push m s = tstack_push m' s'"  *)
+  (* hence 1:  *)
+    (* "Abs_tstack (\<lparr>frame_st = frame_st s, frame_cap = frame_cap s, \<dots> = undefined\<rparr> # Rep_tstack m)  *)
+    (* = Abs_tstack (\<lparr>frame_st = frame_st s', frame_cap = frame_cap s', \<dots> = undefined\<rparr> # Rep_tstack m')" *)
+    (* (is "Abs_tstack ?L = Abs_tstack ?R") *)
+    (* unfolding tstack_push_def by simp *)
+  (* let "?s # Rep_tstack m" = ?L *)
+  (* let "?s' # Rep_tstack m'" = ?R *)
+  (* from 1 have Is_tstack: "Is_tstack ?L" "Is_tstack ?R" "Is_tstack (Rep_tstack m)" "Is_tstack (Rep_tstack m')"  *)
+    (* by auto *)
+  (* hence "?s = ?s'" "Rep_tstack m = Rep_tstack m'" using 1 RepAbs_id list.inject by metis+ *)
+  (* show "s = s'" using \<open>?s = ?s'\<close> using frame.equality frame.ext_inject by (metis (full_types) unit.exhaust) *)
+  (* show "m = m'" using \<open>Rep_tstack m = Rep_tstack m'\<close> Rep_tstack_inject by auto *)
+(* qed *)
 
 abbreviation lifted_abv ("_,_ \<turnstile>\<^sub>s _ {_} _" [20,0,0,0,20] 20)
   where "lifted_abv R G P c Q \<equiv> 
-      srules.rules (tstack_rel (step\<^sub>t R)) (tstack_rel (step G)) (tstack_pred P) (lift\<^sub>c c com.Nil) (tstack_pred Q)" 
+      rules (ts_rel_of_vm_rel (step\<^sub>t R)) (ts_rel_of_vm_rel (step G)) (ts_pred_of_vm_pred P) (lift\<^sub>c c com.Nil) (ts_pred_of_vm_pred Q)" 
+
+term lifted_abv
 
 abbreviation validity_abv  ("\<Turnstile> _ SAT [_, _, _, _]" [60,0,0,0] 45) 
- where "validity_abv c P R G Q \<equiv> srules.validity (lift\<^sub>c c com.Nil) P (tstack_rel (step\<^sub>t R)) (tstack_rel (step G)) Q" 
+ where "validity_abv c P R G Q \<equiv> validity (lift\<^sub>c c com.Nil) P (ts_rel_of_vm_rel (step\<^sub>t R)) (ts_rel_of_vm_rel (step G)) Q" 
 
 text \<open>An ordering property on contexts\<close>
 definition context_order 
@@ -64,24 +111,132 @@ text \<open>The validity property we intend to show, abstracts over the preserva
 definition valid 
   ("_,_ \<turnstile>\<^sub>w _ {_} _" [100,0,0,0,100] 60)
   where "valid R G P c Q \<equiv>  
-     (wellformed R G \<and> stable\<^sub>t R Q \<and> guar\<^sub>c c G) \<longrightarrow> (stable\<^sub>t R P \<and> (R,G \<turnstile>\<^sub>s P {(projectcom c)} Q))" 
+     (wellformed R G \<and> stable\<^sub>t R Q \<and> guar\<^sub>c (vm_lang_of_ts_lang c) G) \<longrightarrow> (stable\<^sub>t R P \<and> (R,G \<turnstile>\<^sub>s P {c} Q))" 
 
+     
+lemma tauxupd_in_ts_pred:
+  assumes "x \<in> ts_pred_of_vm_pred {t. t\<lparr>varmap_rec.more := f t\<rparr> \<in> Q}" 
+  shows "tauxupd x (f \<circ> vm_of_ts) \<in> ts_pred_of_vm_pred Q"
+proof -
+  have "\<exists>t \<in> {t. t\<lparr>varmap_rec.more := f t\<rparr> \<in> Q}. vm_of_ts x = t" using assms ts_of_vm_exists
+    by (simp add: ts_pred_of_vm_pred.rep_eq) 
+  hence Q: "(vm_of_ts x) \<lparr> more := f (vm_of_ts x) \<rparr> \<in> Q" by simp
+
+  have Is_tstack: "Is_tstack (auxupd (Rep_tstack x) (\<lambda>tstack. f (vm_of_ts (Abs_tstack tstack))))"
+    by auto
+  have f: "f (vm_of_ts x) = frame.more (last (Rep_tstack (tauxupd x (f \<circ> vm_of_ts))))"
+    unfolding tauxupd_def 
+    by (auto simp add: Is_tstack, simp add: auxupd_def Rep_tstack_inverse)
+  
+  have "(vm_of_ts x) \<lparr> more := f (vm_of_ts x) \<rparr> = vm_of_ts (tauxupd x (f \<circ> vm_of_ts))"
+  using f unfolding vm_of_ts_def by auto
+
+  thus ?thesis using Q by (simp add: ts_pred_of_vm_pred.abs_eq)
+qed
+
+lemma ts_pred_of_vm_pred_Inter [simp]: 
+  "ts_pred_of_vm_pred (P \<inter> Q) = ts_pred_of_vm_pred P \<inter> ts_pred_of_vm_pred Q"
+unfolding ts_pred_of_vm_pred_def by simp
+
+lemma
+  assumes "ts_rel_of_vm_rel (step\<^sub>t R),ts_rel_of_vm_rel (step G) \<turnstile>\<^sub>A ts_pred_of_vm_pred P {liftg (ts_pred_of_vm_pred c) \<alpha> (f \<circ> vm_of_ts)} ts_pred_of_vm_pred Q"
+  shows "step\<^sub>t R,step G \<turnstile>\<^sub>s P {Op (ts_pred_of_vm_pred c) \<alpha> (f \<circ> vm_of_ts)} Q"
+proof (induct \<alpha>)
+  case (assign x11 x12)
+  have 2: "stable (ts_rel_of_vm_rel (step\<^sub>t R)) (ts_pred_of_vm_pred P)"
+    using assms unfolding atomic_rule_def by simp
+  have 1: "step\<^sub>t (step\<^sub>t R) = step\<^sub>t R" for R unfolding step\<^sub>t_def apply auto sorry
+  show ?case 
+  unfolding assign apply simp apply (rule rules.basic)
+  unfolding atomic_rule_def apply auto
+  unfolding liftg_def apply auto
+  prefer 3 unfolding stable_def 1 apply auto
+  using  2 unfolding stable_def apply auto
+  using assms unfolding atomic_rule_def apply auto 
+  unfolding wp_def liftg_def apply auto
+  prefer 3 apply (meson State.stable_def)
+  defer unfolding guar_def apply auto sorry
+next
+  case (cmp x2)
+  then show ?case sorry
+next
+  case (leak x31 x32)
+  then show ?case sorry
+next
+  case full_fence
+  then show ?case sorry
+next
+  case nop
+  then show ?case sorry
+qed
+     
 section \<open>Soundness\<close>
 
 text \<open>Basic Rule for operations with vc\<close>
 lemma basic_wp\<^sub>i_1:
   assumes "P \<subseteq> stabilize R (c \<inter> wp\<^sub>i \<alpha> (wp\<^sub>a f Q))" "wellformed R G" "stable\<^sub>t R Q" 
   assumes "c \<subseteq> guar (wp\<^sub>i \<alpha> o wp\<^sub>a f) (step G)"
-  shows "(step\<^sub>t R),(step G) \<turnstile>\<^sub>s P {Basic (liftg c \<alpha> f)} Q"
-(*  shows "srules.rules (step\<^sub>t R) (step G) P {Basic (liftg c \<alpha> f)} Q" *)
-(*  shows "(step\<^sub>t R),(step G) \<turnstile> P {Basic (liftg c \<alpha> f)} Q" *)
+  shows "(step\<^sub>t R),(step G) \<turnstile>\<^sub>s P {Op (ts_pred_of_vm_pred c) \<alpha> (f \<circ> vm_of_ts)} Q"
 proof -
-    have "(step\<^sub>t R),(step G) \<turnstile>\<^sub>A (stabilize R (c \<inter> wp\<^sub>i \<alpha> (wp\<^sub>a f Q))) {(liftg c \<alpha> f)} Q"
-(*  have "step\<^sub>t R,step G \<turnstile>\<^sub>A stabilize R (c \<inter> wp\<^sub>i \<alpha> (wp\<^sub>a f Q)) {\<lfloor>c, \<alpha>, f\<rfloor>} Q" *)
-    using assms apply (cases \<alpha>) 
-                by (auto simp: atomic_rule_def guar_def wp_def step_def 
-                                         wp\<^sub>r_def liftg_def o_def  elim!: stabilizeE) 
-  thus ?thesis using assms by (intro conseq[OF basic]) (auto)
+term atomic_rule  
+  have "ts_rel_of_vm_rel (step\<^sub>t R),ts_rel_of_vm_rel(step G) \<turnstile>\<^sub>A ts_pred_of_vm_pred(stabilize R (c \<inter> wp\<^sub>i \<alpha> (wp\<^sub>a f Q))) {(liftg (ts_pred_of_vm_pred c) \<alpha> (f \<circ> vm_of_ts))} ts_pred_of_vm_pred Q"
+  using assms apply (cases \<alpha>) 
+
+  apply (rule atomicI)
+  apply auto
+  proof goal_cases
+  case (1 x11 x12 x)
+  then show ?case sorry
+  next
+  case (2 x11 x12)
+  then show ?case sorry
+  next
+  case (3 x11 x12)
+  then show ?case sorry
+  next
+  case (4 x11 x12)
+  then show ?case sorry
+  next
+  case (5 x2)
+  then show ?case sorry
+  next
+  case (6 x31 x32)
+  then show ?case sorry
+  next
+  case 7
+  then show ?case sorry
+  next
+  case 8
+  then show ?case sorry
+  qed
+    (* case (1 x) *)
+    (* hence x: "x \<in> ts_pred_of_vm_pred (c \<inter> {t. t\<lparr>more := f t\<rparr> \<in> Q})"  *)
+      (* using stabilizeE by (metis (no_types, lifting) ts_pred_of_vm_pred.abs_eq vimageE vimageI) *)
+    (* thus ?case unfolding wp_def liftg_def  *)
+      (* using tauxupd_in_ts_pred by auto *)
+  (* next *)
+    (* case 2 *)
+    (* show ?case unfolding liftg_def State.guar_def apply auto using 2(3) *)
+  (* next *)
+    (* case 3 *)
+    (* then show ?case sorry *)
+  (* next *)
+    (* case 4 *)
+    (* then show ?case sorry *)
+  (* next *)
+    (* case (5 x11 x12) *)
+    (* then show ?case sorry *)
+  (* next *)
+    (* case (6 x2) *)
+    (* then show ?case sorry *)
+  (* next *)
+    (* case (7 x31 x32) *)
+    (* then show ?case sorry *)
+  (* next *)
+    (* case 8 *)
+    (* then show ?case sorry *)
+  (* qed *)
+  thus ?thesis 
 qed
 
 text \<open>Basic Rule for operations without vc\<close>
